moved MU__r to separate file

fairis/heap_lang/examples/even_odd/thread_progs.v
@@ -139,32 +139,6 @@ Section StResImpl.
 End StResImpl. 
 
 
-Definition MU__r `{LM: LiveModel heap_lang M} `{!heapGS Σ LM} ρ E P: iProp Σ :=  
-  ∀ τ f R, τ ↦M ({[ ρ := f ]} ∪ (S <$> R)) ∗ ⌜ ρ ∉ dom R ⌝ -∗
-          MU E τ (τ ↦M ({[ ρ := lm_flm LM ]} ∪ R) ∗ P).
-
-
-Lemma MU__r_wand `{LM: LiveModel heap_lang M} `{!heapGS Σ LM} E ρ (P Q : iProp Σ) :
-  (P -∗ Q) -∗ MU__r ρ E P -∗ MU__r ρ E Q.
-Proof.
-  iIntros "HPQ HMU". rewrite /MU__r. iIntros "**".
-  iSpecialize ("HMU" with "[$]"). 
-  iApply (MU_wand with "[HPQ] [$]"). iFrame.
-  iIntros "[??]". iFrame. by iApply "HPQ". 
-Qed.
-
-
-Lemma MU__r_mask_weaken `{LM: LiveModel heap_lang M} `{!heapGS Σ LM}
-  E1 E2 ρ (P: iProp Σ)
-  (SUB: E1 ⊆ E2):
-  MU__r ρ E1 P -∗ MU__r ρ E2 P.
-Proof.
-  iIntros "MU". rewrite /MU__r. iIntros "**".
-  iApply MU_mask_weaken; eauto.
-  by iApply "MU".
-Qed.
-
-
 Section ProofsGen.  
   Context `{LM__p: LiveModel heap_lang M__p}.
   Context `{!heapGS Σ LM__p}.
