fairis/heap_lang/examples/even_odd/mu_role.v
@@ -1,0 +1,38 @@
+From iris.proofmode Require Import tactics.
+From trillium.fairness Require Import action_model resources fuel.
+From trillium.fairness.heap_lang Require Import notation iris_inst.
+
+
+Section MuRole.
+  Context {AM1 AM2: ActionModel}.
+  Let PM := ProdAM AM1 AM2.
+  Context {PROD_LR: AM_strong_lr PM}. 
+  Let M := AM2FM PM PROD_LR.
+
+  Context {LM: LiveModel heap_lang M}.
+
+  Context `{!heapGS Σ AM1 AM2}. 
+            
+  Definition MU__r ρ E P: iProp Σ :=  
+    ∀ τ f R, τ ↦M ({[ ρ := f ]} ∪ (S <$> R)) ∗ ⌜ ρ ∉ dom R ⌝ -∗
+              MU E τ (τ ↦M ({[ ρ := lm_flm LM ]} ∪ R) ∗ P) (LM := LM).
+
+  Lemma MU__r_wand E ρ (P Q: iProp Σ):
+    (P -∗ Q) -∗ MU__r ρ E P -∗ MU__r ρ E Q.
+  Proof.
+    iIntros "HPQ HMU". rewrite /MU__r. iIntros "**".
+    iSpecialize ("HMU" with "[$]"). 
+    iApply (MU_wand with "[HPQ] [$]"). iFrame.
+    iIntros "[??]". iFrame. by iApply "HPQ". 
+  Qed.
+
+  Lemma MU__r_mask_weaken E1 E2 ρ (P: iProp Σ)
+    (SUB: E1 ⊆ E2):
+    MU__r ρ E1 P -∗ MU__r ρ E2 P.
+  Proof.
+    iIntros "MU". rewrite /MU__r. iIntros "**".
+    iApply MU_mask_weaken; eauto.
+    by iApply "MU".
+  Qed.
+
+End MuRole.
